Gpointers.fst
@@ -39,14 +39,14 @@ assume val ptr_eq:
   q:gpointer a ->
   ST.ST bool
     (requires (fun h -> B.live h p /\ B.live h q))
-    (ensures (fun h0 b h1 -> h0==h1 /\ (b <==> (B.as_addr p = B.as_addr q))))
+    (ensures (fun h0 b h1 -> h0==h1 /\ (b <==> (p == q))))
 
 (** Allow comparing pointers *)
 assume val compare_addrs:
   #a:Type ->
   p:gpointer a ->
   q:gpointer a ->
-  Tot (b:bool{b <==> (B.as_addr p = B.as_addr q)})
+  GTot (b:bool{b <==> (p == q)})
 
 unfold let is_null (p:gpointer_or_null 't) = CN.is_null p
 unfold let is_not_null (p:gpointer_or_null 't) = not (CN.is_null p)
@@ -65,24 +65,28 @@ unfold let ( ! ) (a:gpointer 't) = !* a
 
 unfold let recall (#t:Type) (p: gpointer_or_null t) = recall p
 
-(* We need this for the proof *)
-assume val pointer_live_by_addr (#t:Type0) (h0:HS.mem) (p1 p2:gpointer_or_null t) :
-  Lemma ((h0 `B.live` p1 /\ B.as_addr p1 = B.as_addr p1 /\ is_not_null p2 = is_not_null p2) ==>
-         h0 `B.live` p2)
-    [SMTPat (h0 `B.live` p1); SMTPat (h0 `B.live` p2)] // TODO: Make sure this doesn't over trigger
+/// The commented out part below is a _very_ bad idea, since we _may_
+/// be able to prove false, by taking a ref, freeing it, and having
+/// another allocate to same address, or something similar
 
-val stayin_alive :
-(* Whether you're a brother or whether you're a mother
-   You're stayin' alive, stayin' alive
-   Feel the city breakin' and everybody shakin'
-   I'm a-stayin' alive, stayin' alive
-   Ah, ah, ah, ah, stayin' alive, stayin' alive
-   Ah, ah, ah, ah, stayin' ali-i-i-i-ive *)
-   #t:Type ->
-   h0:HS.mem ->
-   a:gpointer_or_null t ->
-   b:gpointer_or_null t ->
-   Lemma
-     (requires (h0 `B.live` a /\ B.as_addr a = B.as_addr b /\ is_null a = is_null b))
-     (ensures (h0 `B.live` b))
-let stayin_alive #t h0 a b = ()
+// (* We need this for the proof *)
+// assume val pointer_live_by_addr (#t:Type0) (h0:HS.mem) (p1 p2:gpointer_or_null t) :
+//   Lemma ((h0 `B.live` p1 /\ B.as_addr p1 = B.as_addr p1 /\ is_not_null p2 = is_not_null p2) ==>
+//          h0 `B.live` p2)
+//     [SMTPat (h0 `B.live` p1); SMTPat (h0 `B.live` p2)] // TODO: Make sure this doesn't over trigger
+
+// val stayin_alive :
+// (* Whether you're a brother or whether you're a mother
+//    You're stayin' alive, stayin' alive
+//    Feel the city breakin' and everybody shakin'
+//    I'm a-stayin' alive, stayin' alive
+//    Ah, ah, ah, ah, stayin' alive, stayin' alive
+//    Ah, ah, ah, ah, stayin' ali-i-i-i-ive *)
+//    #t:Type ->
+//    h0:HS.mem ->
+//    a:gpointer_or_null t ->
+//    b:gpointer_or_null t ->
+//    Lemma
+//      (requires (h0 `B.live` a /\ B.as_addr a = B.as_addr b /\ is_null a = is_null b))
+//      (ensures (h0 `B.live` b))
+// let stayin_alive #t h0 a b = ()
